new version

src/Distributions/DiscreteLaplace/Equivalence.dfy
@@ -17,130 +17,120 @@ module DiscreteLaplace.Equivalence {
    Definitions
   ************/
 
-  ghost function SampleTailRecursive(scale: Rationals.Rational, b: bool := true, y: int := 0): Monad.Hurd<int>
-    requires scale.numer >= 1
-  {
+  ghost opaque function SampleInnerLoopTailRecursive(x: (bool, int) := (true, 0)): Monad.Hurd<(bool, int)> {
     assume {:axiom} false; // assume termination
     (s: Rand.Bitstream) =>
-      if !(b && y == 0) then
-        Monad.Result(if b then -y else y, s)
+      if x.0 then
+        Monad.Bind(
+          BernoulliExpNeg.Model.Sample(Rationals.Int(1)),
+          (a: bool) => SampleInnerLoopTailRecursive((a, if a then x.1 + 1 else x.1))
+        )(s)
       else
-        var (u, s) :- Uniform.Model.Sample(scale.numer)(s);
-        var (d, s) :- BernoulliExpNeg.Model.Sample(Rationals.Rational(u, scale.numer))(s);
-        if d then
-          var (v, s) :- SampleTailRecursiveHelper(s);
-          var x := u + scale.numer * v;
-          var y := x / scale.denom;
-          var sample := Coin.Model.Sample(s);
-          SampleTailRecursive(scale, sample.value, y)(sample.rest)
-        else
-          SampleTailRecursive(scale, b, y)(s)
-  }
-
-  ghost function SampleTailRecursiveHelper(s: Rand.Bitstream): Monad.Result<int>
-    requires Loops.WhileCutTerminates(Model.SampleHelperLoopCondition, Model.SampleHelperLoopBody, (true, 0), s)
-  {
-    var f := (x: (bool, int)) => x.1;
-    SampleTailRecursiveHelperLoop(s).Map(f)
-  }
-
-  ghost function SampleTailRecursiveHelperLoop(s: Rand.Bitstream, x: (bool, int) := (true, 0)): Monad.Result<(bool, int)>
-    requires Loops.WhileCutTerminates(Model.SampleHelperLoopCondition, Model.SampleHelperLoopBody, x, s)
-  {
-    var fuel := Loops.LeastFuel(Model.SampleHelperLoopCondition, Model.SampleHelperLoopBody, x, s);
-    SampleTailRecursiveHelperLoopCut(x, fuel)(s)
-  }
-
-  ghost function SampleTailRecursiveHelperLoopCut(x: (bool, int) := (true, 0), fuel: nat): Monad.Hurd<(bool, int)>
-    decreases fuel
-  {
-    (s: Rand.Bitstream) =>
-      if fuel == 0 || !x.0 then
-        Monad.Result(x, s)
-      else
-        var (a, s') :- BernoulliExpNeg.Model.Sample(Rationals.Int(1))(s);
-        SampleTailRecursiveHelperLoopCut((a, if a then x.1 + 1 else x.1), fuel - 1)(s')
+        Monad.Return(x)(s)
   }
 
   /*******
    Lemmas
   *******/
 
-  // TODO: add later
-  lemma {:axiom} SampleTailRecursiveEquivalence(scale: Rationals.Rational, s: Rand.Bitstream)
-    requires scale.numer >= 1
-    ensures SampleTailRecursive(scale)(s) == Model.Sample(scale)(s)
-
-  lemma SampleTailRecursiveHelperEquivalence(s: Rand.Bitstream)
-    requires Loops.WhileCutTerminates(Model.SampleHelperLoopCondition, Model.SampleHelperLoopBody, (true, 0), s)
-    ensures SampleTailRecursiveHelper(s) == Model.SampleHelper(s)
+  lemma SampleInnerLoopLiftToEnsures(s: Rand.Bitstream, t: Rand.Bitstream, a: bool, v: int)
+    requires R1: !a 
+    requires R2: SampleInnerLoopTailRecursive()(s) == SampleInnerLoopTailRecursive((a, v))(t)
+    ensures Model.SampleInnerLoopFull()(s) == Monad.Result(v, t)
   {
     var f := (x: (bool, int)) => x.1;
+
+    assert A: Model.SampleInnerLoop()(s) == Monad.Result((a, v), t) by {
+      calc {
+        Model.SampleInnerLoop()(s);
+        Model.SampleInnerLoop((true, 0))(s);
+        { SampleInnerLoopTailRecursiveEquivalence(s); }
+        SampleInnerLoopTailRecursive((true, 0))(s);
+        SampleInnerLoopTailRecursive()(s);
+        { reveal R2; }
+        SampleInnerLoopTailRecursive((a, v))(t);
+        { reveal SampleInnerLoopTailRecursive(); reveal R1; }
+        Monad.Return((a, v))(t);
+        Monad.Result((a, v), t);
+      }
+    }
+
     calc {
-      SampleTailRecursiveHelper(s);
-      SampleTailRecursiveHelperLoop(s).Map(f);
-      if SampleTailRecursiveHelperLoop(s).Diverging? then Monad.Diverging else Monad.Result(f(SampleTailRecursiveHelperLoop(s).value), SampleTailRecursiveHelperLoop(s).rest);
-      { SampleTailRecursiveHelperEquivalence2((true, 0), s); }
-      if Model.SampleHelperLoop(s).Diverging? then Monad.Diverging else Monad.Result(f(Model.SampleHelperLoop(s).value), Model.SampleHelperLoop(s).rest);
-      Model.SampleHelperLoop(s).Map(f);
-      Model.SampleHelper(s);
+      Model.SampleInnerLoopFull()(s);
+      Model.SampleInnerLoop()(s).Map(f);
+      { reveal A; }
+      Monad.Result((a, v), t).Map(f);
+      Monad.Result(v, t);
     }
   }
 
-  lemma SampleTailRecursiveHelperEquivalence2(x: (bool, int), s: Rand.Bitstream)
-    requires Loops.WhileCutTerminates(Model.SampleHelperLoopCondition, Model.SampleHelperLoopBody, x, s)
-    ensures SampleTailRecursiveHelperLoop(s, x) == Model.SampleHelperLoop(s, x)
-  {
-    var fuel := Loops.LeastFuel(Model.SampleHelperLoopCondition, Model.SampleHelperLoopBody, x, s);
+  lemma SampleInnerLoopTailRecursiveEquivalence(s: Rand.Bitstream, x: (bool, int) := (true, 0))
+    decreases s
+    ensures Model.SampleInnerLoop(x)(s) == SampleInnerLoopTailRecursive(x)(s)
+  { 
+    var r := Model.SampleInnerLoopBody(x)(s);
+    Model.SampleInnerLoopTerminatesAlmostSurely();
+
     calc {
-      SampleTailRecursiveHelperLoop(s, x);
-      SampleTailRecursiveHelperLoopCut(x, fuel)(s);
-      { SampleTailRecursiveHelperEquivalence3(x, s, fuel); }
-      Loops.WhileCut(Model.SampleHelperLoopCondition, Model.SampleHelperLoopBody, x, fuel)(s);
-      { reveal Loops.While(); }
-      Loops.While(Model.SampleHelperLoopCondition, Model.SampleHelperLoopBody)(x)(s);
-      Model.SampleHelperLoop(s, x);
+      Model.SampleInnerLoop(x)(s);
+    == { reveal Loops.While(); }
+      Loops.While(Model.SampleInnerLoopCondition, Model.SampleInnerLoopBody)(x)(s);
+    ==  { Loops.WhileUnroll(Model.SampleInnerLoopCondition, Model.SampleInnerLoopBody, x, s); }
+      if Model.SampleInnerLoopCondition(x) then 
+        Monad.Bind(Model.SampleInnerLoopBody(x), (y: (bool, int)) => Model.SampleInnerLoop(y))(s)
+      else
+        Monad.Return(x)(s);
+    == { reveal Model.SampleInnerLoopCondition();  }
+      if x.0 then 
+        if r.Result? then Model.SampleInnerLoop(r.value)(r.rest) else Monad.Diverging
+      else 
+        Monad.Return(x)(s);
+    == { if r.Result? { SampleInnerLoopTailRecursiveEquivalence(r.rest, r.value); } }
+      if x.0 then 
+        if r.Result? then SampleInnerLoopTailRecursive(r.value)(r.rest) else Monad.Diverging
+      else 
+        Monad.Return(x)(s);
+    ==
+      if x.0 then 
+        Monad.Bind(Model.SampleInnerLoopBody(x), SampleInnerLoopTailRecursive)(s)
+      else 
+        Monad.Return(x)(s);
+    ==
+      if x.0 then 
+        Monad.Bind(
+          Monad.Bind(
+            BernoulliExpNeg.Model.Sample(Rationals.Int(1)), 
+            (a: bool) => Monad.Return((a, if a then x.1 + 1 else x.1))
+          ),
+          SampleInnerLoopTailRecursive
+        )(s)
+      else 
+        Monad.Return(x)(s);
+    ==
+      if x.0 then 
+        Monad.Bind(
+          BernoulliExpNeg.Model.Sample(Rationals.Int(1)), 
+          (a: bool) => 
+            Monad.Bind(
+              Monad.Return((a, if a then x.1 + 1 else x.1)),
+              SampleInnerLoopTailRecursive
+            )
+        )(s)
+      else 
+        Monad.Return(x)(s);
+    == 
+      if x.0 then
+        Monad.Bind(
+          BernoulliExpNeg.Model.Sample(Rationals.Int(1)),
+          (a: bool) => SampleInnerLoopTailRecursive((a, if a then x.1 + 1 else x.1))
+        )(s)
+      else
+        Monad.Return(x)(s);
+    == { reveal SampleInnerLoopTailRecursive();  }
+      SampleInnerLoopTailRecursive(x)(s);
     }
   }
 
-  lemma SampleTailRecursiveHelperEquivalence3(x: (bool, int), s: Rand.Bitstream, fuel: nat)
-    decreases fuel
-    ensures SampleTailRecursiveHelperLoopCut(x, fuel)(s) == Loops.WhileCut(Model.SampleHelperLoopCondition, Model.SampleHelperLoopBody, x, fuel)(s)
-  {
-    if !x.0 {
-      calc {
-        SampleTailRecursiveHelperLoopCut(x, fuel)(s);
-        Monad.Return(x)(s);
-        Loops.WhileCut(Model.SampleHelperLoopCondition, Model.SampleHelperLoopBody, x, fuel)(s);
-      }
-    } else if fuel == 0 {
-      calc {
-        SampleTailRecursiveHelperLoopCut(x, fuel)(s);
-        Monad.Return(x)(s);
-        Loops.WhileCut(Model.SampleHelperLoopCondition, Model.SampleHelperLoopBody, x, fuel)(s);
-      }
-    } else {
-      var r := Model.SampleHelperLoopBody(x)(s);
-      if r.Result? {
-        var (x', s') := Model.SampleHelperLoopBody(x)(s).Extract();
-        calc {
-          SampleTailRecursiveHelperLoopCut(x, fuel)(s);
-          Monad.Bind(Model.SampleHelperLoopBody(x), (x': (bool, int)) => SampleTailRecursiveHelperLoopCut(x', fuel - 1))(s);
-          SampleTailRecursiveHelperLoopCut(x', fuel - 1)(s');
-          { SampleTailRecursiveHelperEquivalence3(x', s', fuel - 1); }
-          Loops.WhileCut(Model.SampleHelperLoopCondition, Model.SampleHelperLoopBody, x', fuel - 1)(s');
-          Monad.Bind(Model.SampleHelperLoopBody(x), (x': (bool, int)) => Loops.WhileCut(Model.SampleHelperLoopCondition, Model.SampleHelperLoopBody, x', fuel - 1))(s);
-          Loops.WhileCut(Model.SampleHelperLoopCondition, Model.SampleHelperLoopBody, x, fuel)(s);
-        }
-      } else {
-        calc {
-          SampleTailRecursiveHelperLoopCut(x, fuel)(s);
-          Monad.Bind(Model.SampleHelperLoopBody(x), (x': (bool, int)) => SampleTailRecursiveHelperLoopCut(x', fuel - 1))(s);
-          Monad.Diverging;
-          Monad.Bind(Model.SampleHelperLoopBody(x), (x': (bool, int)) => Loops.WhileCut(Model.SampleHelperLoopCondition, Model.SampleHelperLoopBody, x', fuel - 1))(s);
-          Loops.WhileCut(Model.SampleHelperLoopCondition, Model.SampleHelperLoopBody, x, fuel)(s);
-        }
-      }
-    }
-  }
+
+
 }
